Db/Backends/PostgreSQL/Interpretation.lean
@@ -4,6 +4,7 @@ Released under Apache 2.0 license as described in the file LICENSE.
 Authors: Christian Merten
 -/
 import Db.Backends.PostgreSQL.Basic
+import Db.Utils.FromString
 import Db.Backends.Sql
 import Db.Interpretation.Basic
 
@@ -28,17 +29,63 @@ structure State where
 
 abbrev M := ExceptT Exception (StateT State IO)
 
+nonrec def M.run (s : State) {α : Type} (x : M α) : IO (Except Exception α) := do
+  return (← x.run.run s).1
+
+def runDB (connectionInfo : String) {α : Type} (x : M α) : IO (Except Exception α) := do
+  let conn ← connect connectionInfo
+  match conn with
+  | some conn => x.run { connectionInfo := connectionInfo, connection := conn }
+  | none => return .error .fatal
+
 instance (d : Database) : DBMonad d M where
   lookup {names} q := do
     let conn := (← get).connection
     let sql : SQL.Select := .fromQuery q
     let res ← conn.exec sql.toString
     match res with
-    | .data data => data.rows.mapM <| fun map ↦ do
+    | .data data =>
+        data.rawRows.mapM <| fun row ↦ do
+          let mut map := default
+          for name in names do
+            if h : name.toString ∈ row then do
+              let x := row[name.toString]
+              match (FromString.fromString row[name.toString] :
+                  Option name.dbtype.Value) with
+              | some val => map := map.insert name val
+              | none => pure ()
+            else
+              pure ()
+          return map
+        --let mut rows := #[]
+        --for i in Fin.range data.nrows do
+        --  let row : Std.DHashMap d.Name fun n => n.dbtype.Value ← do
+        --    let mut map := default
+        --    for name in names do
+        --      map := map.insert name _
+        --    pure map
+        --  rows := rows.push row
+        --return rows
+    | _ => throw .fatal
+
+/-
+    data.rows.mapM <| fun map ↦ do
         let mut result := .emptyWithCapacity
-        for pair in map do
-          result := result.insert sorry sorry
+        for (name, value) in map do
+          match name.splitOn "." with
+          | [tableName, columnName] =>
+              match d.resolveName tableName columnName with
+              | some (.ident i) =>
+                match value with
+                | .raw s => _
+                | .int n => _
+                | .bool b => result := result.insert (.ident i) (unsafeCast b)
+                | .string s => result := result.insert (.ident i) (unsafeCast s)
+                --have heq : (Database.Name.ident i).dbtype.Value = VarChar 100 := sorry
+                --result := result.insert (.ident i) sorry
+              | _ => pure ()
+          | _ => pure ()
         return result
-    | _ => sorry
+    -/
 
 end PostgreSQL
