Db/Utils/FromString.lean
@@ -1,0 +1,2 @@
+class FromString (α : Type) where
+  fromString : String → Option α
